rt riscv refine: update after adding ct_activatable'_asrt to schedule
Signed-off-by: Michael McInerney <michael.mcinerney@proofcraft.systems>

proof/refine/RISCV64/Invariants_H.thy
@@ -1117,6 +1117,9 @@ abbreviation
 abbreviation
   "activatable' st \<equiv> runnable' st \<or> idle' st"
 
+defs ct_activatable'_asrt_def:
+  "ct_activatable'_asrt \<equiv> ct_in_state' activatable'"
+
 defs rct_imp_activatable'_asrt_def:
   "rct_imp_activatable'_asrt \<equiv> \<lambda>s. ksSchedulerAction s = ResumeCurrentThread \<longrightarrow>
                                          ct_in_state' activatable' s"
